backends/lean/Aeneas/Inv/Test.lean
@@ -13,29 +13,19 @@ def analyzeLoop (k : Array (FVarId × Var) → Expr → State → TacticM α) : 
   trace[Inv] "{tgt}"
   -- Dive into the loop
   let args := tgt.consumeMData.getAppArgs
-  if args.size ≠ 2 then throwError "Expected two arguments, got: {args}"
-  let body := args[1]!
-  -- Dive into the lambdas
-  Meta.lambdaTelescope body.consumeMData fun inputFVars body => do
-  trace[Inv] "inputs: {inputFVars}"
-  let (inputVars, state) ← State.init 0 inputFVars
-  trace[Inv] "initial state: {state}"
-  let (_, state) ← FootprintM.run (footprint.expr true body) state
-  trace[Inv] "{state}"
-  k inputVars body state
+  if h: args.size ≠ 3 then throwError "Expected 3 arguments, got: {args}"
+  else
+    let body := args[1]
+    let (inputVars, state) ← State.init 0 0 #[]
+    let (_, state) ← FootprintM.run (footprint.expr none body) state
+    trace[Inv] "{state}"
+    k inputVars body state
 
 elab "analyze_loop" : tactic => do
-  analyzeLoop fun _ _ _ => pure ()
-
-scoped syntax "analyze_loopiter" : tactic
-
-elab "analyze_loopIter" : tactic => do
-  analyzeLoop fun inputVars _body state => do
-  let output := analyzeFootprint state.toFootprint inputVars[1]!.snd
-  trace[Inv] "Analyzed output:\n{output}"
+  analyzeLoop fun _ _body state => do
+  let output := analyzeFootprint state.toFootprint {}
+  trace[Inv] "Analyzed output:\n{output.map Std.HashMap.toArray}"
   pure ()
-
-def loop (_ : α) : Prop := True
 
 attribute [inv_array_getter xs at i] getElem!
 attribute [inv_array_getter xs at i] getElem
@@ -47,64 +37,101 @@ attribute [inv_val val] Fin.mk
 attribute [inv_val 3] pure
 attribute [inv_val x] Id.run
 
+@[inv_loop_iter {_body} [_start:_stop: += 1] input]
+def loopIter {α} (_start _stop : Nat) (input : α) (_body : Nat → α → α) : α := input
+
+@[inv_loop_iter {_body} [_start:stop: += 1] input]
+def loopIterFin {α} (_start stop : Nat) (input : α) (_body : Fin stop → α → α) : α := input
+
+@[inv_loop_iter {_body} [_start:stop: += 1] input]
+def loopIterFinId {α} (_start stop : Nat) (input : α) (_body : Fin stop → α → Id α) : Id α := input
+
+def post : α → (α → Prop) → Prop := fun _ _ => True
+
+-- No loop
 set_option trace.Inv true in
-example : loop (fun (x y : Array Nat) => (x.set! 0 x[0]!, y)) := by
+example :
+  post 0
+    (fun _ => True)
+  := by
   analyze_loop
-  simp [loop]
+  simp [post]
 
+-- Simple loop
 set_option trace.Inv true in
-example : loop (fun (x y : Array Nat) => (x.set! 0 x.toList[0]!, y)) := by
+example :
+  post (
+    loopIter 0 256 #[]
+      fun i (x : Array Nat) =>
+      x.set! i 0)
+    (fun _ => True)
+  := by
   analyze_loop
-  simp [loop]
-
-def loopIter (_ : Nat → α → α) : Prop := True
-
-set_option trace.Inv true in
-@[inv_loop_iter {_body} [_start:_stop: += 1] _input]
-def loopIterRange {α} (_body : Nat → α → α) (_start _stop : Nat) (_input : α) : Prop := True
+  simp [post]
 
 -- Tuple projectors
 set_option trace.Inv true in
-example : loopIter (fun i (xy : Array Nat × Array Nat) =>
-  let x := xy.fst
-  let y := xy.snd
-  (x.set! i x[i]!, y.set! i x[i]!)) := by
-  analyze_loopIter
-  simp [loopIter]
+example :
+  post (
+    loopIter 0 256 (#[], #[])
+      fun i (xy : Array Nat × Array Nat) =>
+      let x := xy.fst
+      let y := xy.snd
+      (x.set! i x[i]!, y.set! i x[i]!))
+    (fun _ => True)
+  := by
+  analyze_loop
+  simp [post]
 
 -- Tuple with 2 elements
 set_option trace.Inv true in
-example : loopIter (fun i (xy : Array Nat × Array Nat) =>
-  let (x, y) := xy
-  (x.set! i x[i]!, y)) := by
-  analyze_loopIter
-  simp [loopIter]
+example :
+  post (
+    loopIter 0 256 (#[], #[]) (fun i (xy : Array Nat × Array Nat) =>
+      let (x, y) := xy
+      (x.set! i x[i]!, y)))
+    (fun _ => True)
+  := by
+  analyze_loop
+  simp [post]
 
 -- Tuple with 2 elements: checking that the constructor is handled properly
 set_option trace.Inv true in
-example : loopIter (fun i (xy : Array Nat × Array Nat) =>
-  let (x, y) := xy
-  let xy := (x, y)
-  let (x, y) := xy
-  (x.set! i x[i]!, y)) := by
-  analyze_loopIter
-  simp [loopIter]
+example :
+  post (
+    loopIter 0 256 (#[], #[])
+    fun i (xy : Array Nat × Array Nat) =>
+    let (x, y) := xy
+    let xy := (x, y)
+    let (x, y) := xy
+    (x.set! i x[i]!, y))
+  (fun _ => True) := by
+  analyze_loop
+  simp [post]
 
 -- `MProd` with 2 elements: checking that the constructor is handled properly
 set_option trace.Inv true in
-example : loopIter (fun i (xy : MProd (Array Nat) (Array Nat)) =>
-  let ⟨ x, y ⟩ := xy
-  ⟨ x.set! i x[i]!, y ⟩) := by
-  analyze_loopIter
-  simp [loopIter]
+example :
+  post (
+    loopIter 0 256 ⟨#[], #[]⟩
+      fun i (xy : MProd (Array Nat) (Array Nat)) =>
+      let ⟨ x, y ⟩ := xy
+      ⟨ x.set! i x[i]!, y ⟩)
+    (fun _ => True) := by
+  analyze_loop
+  simp [post]
 
 -- Tuple with 3 elements (make sure the handling of tuples is general)
 set_option trace.Inv true in
-example : loopIter (fun i (xyz : Array Nat × Array Nat × Array Nat) =>
-  let (x, y, z) := xyz
-  (x.set! i x[i]!, y, z)) := by
-  analyze_loopIter
-  simp [loopIter]
+example :
+  post (
+    loopIter 0 256 (#[], #[], #[])
+      fun i (xyz : Array Nat × Array Nat × Array Nat) =>
+      let (x, y, z) := xyz
+      (x.set! i x[i]!, y, z))
+    (fun _ => True) := by
+  analyze_loop
+  simp [post]
 
 inductive Either (α β : Type)
 | left  : α → Either α β
@@ -112,74 +139,98 @@ inductive Either (α β : Type)
 
 -- Just checking that we don't crash on arbitrary match expressions
 set_option trace.Inv true in
-example {α β} : loop (fun (e : Either α β) =>
-  match e with
-  | .left _ => true
-  | .right _ => false) := by
+example :
+  post (
+    loopIter 0 256 (Either.left 32) (fun _ (e : Either Nat Nat) =>
+      match e with
+      | .left x => Either.right x
+      | .right y => Either.left y))
+    (fun _ => True) := by
   analyze_loop
-  simp [loop]
+  simp [post]
 
 -- Basic operations: map i
 set_option trace.Inv true in
-example : loopIter (fun i (state : Array Nat × Array Nat) =>
-  let (src, dst) := state
-  let a := src[i]! + dst[i]!
-  let src' := src.set! i 0
-  let dst := dst.set! i a
-  (src', dst)) := by
-  analyze_loopIter
-  simp [loopIter]
+example :
+  post (
+    loopIter 0 256 (#[], #[])
+      fun i (state : Array Nat × Array Nat) =>
+      let (src, dst) := state
+      let a := src[i]! + dst[i]!
+      let src' := src.set! i 0
+      let dst := dst.set! i a
+      (src', dst))
+    (fun _ => True)
+     := by
+  analyze_loop
+  simp [post]
 
 -- Basic operations: 2 * i, 2 * i + 1
 set_option trace.Inv true in
-example : loopIter (fun i (state : Array Nat × Array Nat) =>
-  let (src, dst) := state
-  let a := src[2 * i]! + dst[2 * i]!
-  let b := src[2 * i + 1]! + dst[2 * i + 1]!
-  let src := src.set! (2 * i) 0
-  let src := src.set! (2 * i + 1) 0
-  let dst := dst.set! (2 * i) a
-  let dst := dst.set! (2 * i + 1) b
-  (src, dst)) := by
-  analyze_loopIter
-  simp [loopIter]
+example :
+  post (
+    loopIter 0 256 (#[], #[])
+      fun i (state : Array Nat × Array Nat) =>
+      let (src, dst) := state
+      let a := src[2 * i]! + dst[2 * i]!
+      let b := src[2 * i + 1]! + dst[2 * i + 1]!
+      let src := src.set! (2 * i) 0
+      let src := src.set! (2 * i + 1) 0
+      let dst := dst.set! (2 * i) a
+      let dst := dst.set! (2 * i + 1) b
+      (src, dst))
+    (fun _ => True) := by
+  analyze_loop
+  simp [post]
 
 -- We are not limited to `Nat`: the following loop uses `Fin`
 set_option trace.Inv true in
-example : loop (fun (i : Fin 32) (state : Array Nat × Array Nat) =>
-  let (src, dst) := state
-  let j := Fin.mk i.val i.isLt -- create a new `Fin` equal to `i`
-  let a := src[2 * j]! + dst[2 * j]!
-  let b := src[2 * j + 1]! + dst[2 * j + 1]!
-  let src := src.set! (2 * j) 0
-  let src := src.set! (2 * j + 1) 0
-  let dst := dst.set! (2 * j) a
-  let dst := dst.set! (2 * j + 1) b
-  (src, dst)) := by
-  analyze_loopIter
-  simp [loop]
+example :
+  post (
+    loopIterFin 0 32 (#[], #[])
+      fun (i : Fin 32) (state : Array Nat × Array Nat) =>
+      let (src, dst) := state
+      let j := Fin.mk i.val i.isLt -- create a new `Fin` equal to `i`
+      let a := src[2 * j]! + dst[2 * j]!
+      let b := src[2 * j + 1]! + dst[2 * j + 1]!
+      let src := src.set! (2 * j) 0
+      let src := src.set! (2 * j + 1) 0
+      let dst := dst.set! (2 * j) a
+      let dst := dst.set! (2 * j + 1) b
+      (src, dst))
+    (fun _ => True) := by
+  analyze_loop
+  simp [post]
 
 -- Monadic binds: state has one array
 set_option trace.Inv true in
-example : loopIter (fun (i : Nat) (a : Array Nat) => Id.run do
-  let a ← a.set! i 0
-  pure a) := by
-  analyze_loopIter
-  simp [loopIter]
+example :
+  post (
+    loopIter 0 256 #[]
+      fun (i : Nat) (a : Array Nat) => Id.run do
+      let a ← a.set! i 0
+      pure a)
+    (fun _ => True) := by
+  analyze_loop
+  simp [post]
 
 -- Monadic bind: state is a tuple of arrays
 set_option trace.Inv true in
-example : loop (fun (i : Fin 32) (state : Array Nat × Array Nat) => Id.run do
-  let (src, dst) ← state
-  let j ← Fin.mk i.val i.isLt
-  let a ← src[2 * j]! + dst[2 * j]!
-  let b ← src[2 * j + 1]! + dst[2 * j + 1]!
-  let src ← src.set! (2 * j) 0
-  let src ← src.set! (2 * j + 1) 0
-  let dst ← dst.set! (2 * j) a
-  let dst ← dst.set! (2 * j + 1) b
-  pure (src, dst)) := by
-  analyze_loopIter
-  simp [loop]
+example :
+  post (
+    loopIterFinId 0 32 (#[], #[])
+      fun (i : Fin 32) (state : Array Nat × Array Nat) => do
+      let (src, dst) ← state
+      let j ← Fin.mk i.val i.isLt
+      let a ← src[2 * j]! + dst[2 * j]!
+      let b ← src[2 * j + 1]! + dst[2 * j + 1]!
+      let src ← src.set! (2 * j) 0
+      let src ← src.set! (2 * j + 1) 0
+      let dst ← dst.set! (2 * j) a
+      let dst ← dst.set! (2 * j + 1) b
+      pure (src, dst))
+    (fun _ => True) := by
+  analyze_loop
+  simp [post]
 
 end Aeneas.Inv.Test
